proving in ElimDead.v

platform/cito/ElimDead.v
@@ -1,20 +1,40 @@
 Require Import Syntax.
 Import String Memory IL SyntaxExpr.
 Require Import Notations.
+Require Import Equalities SetModule.
 
 Set Implicit Arguments.
 
-Variable set : Type.
-Variable mem_dec : string -> set -> bool.
+Module Key <: MiniDecidableType.
+  Definition t := string.
+  Definition eq_dec := string_dec.
+End Key.
+
+Module MSet := ArrowSet Key.
+Import MSet.
+
 Variable remove : set -> string -> set.
 Infix "%-" := remove (at level 20).
-Variable free_vars : Expr -> set.
-Variable free_vars_stmt : Statement -> set.
+Variable used_vars : Expr -> set.
 Notation skip := Syntax.Skip.
-Variable union : set -> set -> set.
-Infix "+" := union.
 
 Open Scope stmnt.
+Open Scope set.
+
+Fixpoint used_vars_stmt s :=
+  match s with
+    | skip => {}
+    | a ;: b => used_vars_stmt a + used_vars_stmt b
+    | Conditional e t f => used_vars e + used_vars_stmt t + used_vars_stmt f
+    | Loop e body => used_vars e + used_vars_stmt body
+    | x <- e => used_vars e
+    | x <== arr[idx] => used_vars arr + used_vars idx
+    | arr[idx] <== e => used_vars arr + used_vars idx + used_vars e
+    | x <- new e => used_vars e
+    | Free e => used_vars e
+    | Len x e => used_vars e
+    | Call f[x] => used_vars f + used_vars x
+  end.
 
 Fixpoint elim_dead s used : Statement * set :=
   match s with
@@ -34,40 +54,188 @@ Fixpoint elim_dead s used : Statement * set :=
       let result := elim_dead f used in
       let f := fst result in
       let used_f := snd result in
-      (Conditional e t f, free_vars e + used_t + used_f)
+      (Conditional e t f, used_vars e + used_t + used_f)
     | Loop e body => 
-      let result := elim_dead body (used + free_vars e + free_vars_stmt body) in
+      let result := elim_dead body (used + used_vars e + used_vars_stmt body) in
       let body := fst result in
       let used' := snd result in
-      (Loop e body, used + used' + free_vars e)
+      (Loop e body, used + used' + used_vars e)
     | x <- e =>
       if mem_dec x used then
-        (s, used %- x + free_vars e)
+        (s, used %- x + used_vars e)
       else
         (skip, used)
     | x <== arr[idx] =>
-      if mem_dec x used then
-        (s, used %- x + free_vars arr + free_vars idx)
-      else
-        (skip, used)
+      (s, used %- x + used_vars arr + used_vars idx)
     | arr[idx] <== e =>
-      (s, used + free_vars arr + free_vars idx + free_vars e)
+      (s, used + used_vars arr + used_vars idx + used_vars e)
     | x <- new e =>
-      (s, used %- x + free_vars e)
+      (s, used %- x + used_vars e)
     | Free e =>
-      (s, used + free_vars e)
+      (s, used + used_vars e)
     | Len x e =>
-      if mem_dec x used then
-        (s, used %- x + free_vars e)
-      else
-        (skip, used)
+      (s, used %- x + used_vars e)
     | Call f[x] =>
-      (s, used + free_vars f + free_vars x)
+      (s, used + used_vars f + used_vars x)
   end.
 
 Require Import Semantics.
 
-Variable agree_in : vals -> vals -> set -> Prop.
+Definition agree_in a b s := forall x, x %in s -> Locals.sel a x = Locals.sel b x.
+
+Ltac openhyp' :=
+  repeat match goal with
+           | H : context [mem_dec ?A ?B] |- _ => destruct (mem_dec A B)
+           | |- context [mem_dec ?A ?B] => destruct (mem_dec A B)
+           | H : context [ { _ | _ } ] |- _ => destruct H
+         end.
+
+Ltac unfold_all :=
+  repeat match goal with
+           | H := _ |- _ => unfold H in *; clear H
+         end.
+
+Require Import GeneralTactics.
+Import SemanticsExpr.
+Notation eval := exprDenote.
+
+Lemma eval_agree_in : forall e a b, agree_in a b (used_vars e) -> eval e a = eval e b.
+  admit.
+Qed.
+
+Lemma upd_same_agree_in : forall a b s x w, agree_in a b (s %- x) -> agree_in (upd a x w) (upd b x w) s.
+  admit.
+Qed.
+
+Lemma agree_in_subset : forall a b s s', agree_in a b s -> (s' <= s)%set -> agree_in a b s'.
+  admit.
+Qed.
+
+Lemma upd_out_agree_in : forall a b s x w, agree_in a b s -> ~ x %in s -> agree_in (upd a x w) b s.
+  admit.
+Qed.
+
+Hint Constructors RunsTo.
+Hint Resolve subset_union_1 subset_union_2.
+
+Open Scope set_scope.
+
+Lemma union_subset : forall (a b c : set), a <= c -> b <= c -> a + b <= c.
+  admit.
+Qed.
+
+Variable add : set -> string -> set.
+Infix "%+" := add (at level 20).
+
+Lemma add_subset_union : forall a x, a %+ x <= a + singleton x.
+  admit.
+Qed.
+
+Lemma union_subset_add : forall a x, a + singleton x <= a %+ x.
+  admit.
+Qed.
+
+Definition subset_union_left : forall a b, a <= a + b.
+  admit.
+Qed.
+
+Definition subset_union_right : forall a b, b <= a + b.
+  admit.
+Qed.
+
+Definition subset_trans : forall a b c, a <= b -> b <= c -> a <= c.
+  admit.
+Qed.
+
+Definition remove_subset : forall a x, a %- x <= a.
+  admit.
+Qed.
+
+Ltac subset_solver :=
+  repeat 
+    match goal with
+      | |- ?A <= ?A => eapply subset_refl
+      | |- _ + _ <= _ => eapply union_subset
+      | |- ?S <= ?A + _ =>
+        match A with
+            context [ S ] => eapply subset_trans; [ .. | eapply subset_union_left]
+        end
+      | |- ?S <= _ + ?B =>
+        match B with
+            context [ S ] => eapply subset_trans; [ .. | eapply subset_union_right]
+        end
+      | |- _ %+ _ <= _ => eapply subset_trans; [ eapply add_subset_union | .. ]
+      | |- _ <= _ %+ _ => eapply subset_trans; [ .. | eapply union_subset_add ]
+      | |- _ %- _ <= _ => eapply subset_trans; [ eapply remove_subset | .. ]
+      end.
+
+Hint Extern 0 (subset _ _) => progress subset_solver.
+
+Hint Resolve upd_same_agree_in.
+Hint Resolve agree_in_subset.
+Hint Resolve upd_out_agree_in.
+
+Lemma agree_in_symm : forall a b s, agree_in a b s -> agree_in b a s.
+  admit.
+Qed.
+Hint Resolve agree_in_symm.
+
+Lemma elim_dead_upper_bound : 
+  forall s used,
+    let result := elim_dead s used in
+    let used' := snd result in
+    used' <= used + used_vars_stmt s.
+Proof.
+  induction s; simpl; intuition eauto using subset_trans.
+  openhyp'; simpl in *; eauto.
+Qed.
+Hint Resolve elim_dead_upper_bound.
+
+Lemma while_case :
+  forall fs t v v',
+    RunsTo fs t v v' ->
+    forall e body used vs,
+      let s := Loop e body in
+      let result := elim_dead s used in
+      let s' := fst result in
+      let used' := snd result in
+      let vt := fst v in
+      let heap := snd v in
+      let vt' := fst v' in
+      let heap' := snd v' in
+      t = s' ->
+      agree_in vs vt used' ->
+      (
+        let s := body in
+
+        forall (used : set) (vs vt : vals) (heap : arrays) 
+               (vt' : vals) (heap' : arrays),
+          let result := elim_dead s used in
+          let t := fst result in
+          let used' := snd result in
+          RunsTo fs t (vt, heap) (vt', heap') ->
+          agree_in vs vt used' ->
+          exists vs' : vals,
+            RunsTo fs s (vs, heap) (vs', heap') /\ agree_in vs' vt' used
+      ) ->
+      exists vs',
+        RunsTo fs s (vs, heap) (vs', heap) /\
+        agree_in vs' vt' used.
+Proof.
+  induction 1; simpl; intros; unfold_all; subst; intuition.
+
+  injection H2; intros; subst.
+  destruct v; simpl in *.
+  destruct v'; simpl in *.
+  eapply H4 in H0; eauto; openhyp.
+  destruct v''; simpl in *.
+  edestruct IHRunsTo2; try reflexivity.
+  2 : eauto.
+  eauto using subset_trans.
+  openhyp.
+  descend.
+(*here*)
+  eauto.
 
 Lemma elim_dead_is_bp : 
   forall fs s used vs vt heap vt' heap', 
@@ -79,4 +247,112 @@ Lemma elim_dead_is_bp :
     exists vs',
       RunsTo fs s (vs, heap) (vs', heap') /\
       agree_in vs' vt' used.
-    
+Proof.
+  induction s; simpl; intros.
+
+  openhyp'; simpl in *.
+  inversion H; unfold_all; subst.
+  descend; intuition.
+  erewrite eval_agree_in by eauto.
+  eauto.
+
+  inversion H; unfold_all; subst.
+  descend; intuition.
+
+  inversion H; unfold_all; subst.
+  descend.
+  econstructor.
+  repeat erewrite (@eval_agree_in _ vs vt) by eauto.
+  eauto.
+  repeat erewrite (@eval_agree_in _ vs vt) by eauto.
+  eauto.
+
+  inversion H; unfold_all; subst.
+  descend; intuition.
+  repeat erewrite (@eval_agree_in _ vt' vs) by eauto.
+  econstructor.
+  repeat erewrite (@eval_agree_in _ vs vt') by eauto.
+  eauto.
+  eauto.
+  
+  inversion H; unfold_all; subst.
+  destruct v'; simpl in *.
+  eapply IHs1 in H3; eauto; openhyp.
+  eapply IHs2 in H6; eauto; openhyp.
+  descend.
+  eauto.
+  eauto.
+
+  inversion H; unfold_all; subst.
+  descend.
+  eauto.
+  eauto.
+
+  inversion H; unfold_all; subst.
+  simpl in *.
+  eapply IHs1 in H7; eauto; openhyp.
+  descend.
+  econstructor.
+  simpl.
+  repeat erewrite (@eval_agree_in _ vs vt) by eauto.
+  eauto.
+  eauto.
+  eauto.
+
+  simpl in *.
+  eapply IHs2 in H7; eauto; openhyp.
+  descend.
+  econstructor 7.
+  simpl.
+  repeat erewrite (@eval_agree_in _ vs vt) by eauto.
+  eauto.
+  eauto.
+  eauto.
+
+  admit.
+
+  inversion H; unfold_all; subst.
+  descend.
+  econstructor.
+  eauto.
+  repeat erewrite (@eval_agree_in _ vs vt) by eauto.
+  eauto.
+  repeat erewrite (@eval_agree_in _ vs vt) by eauto.
+  eauto.
+  eauto.
+
+  inversion H; unfold_all; subst.
+  descend.
+  repeat erewrite (@eval_agree_in _ vt' vs) by eauto.
+  econstructor.
+  repeat erewrite (@eval_agree_in _ vs vt') by eauto.
+  eauto.
+  eauto.
+
+  inversion H; unfold_all; subst.
+  descend.
+  econstructor.
+  repeat erewrite (@eval_agree_in _ vs vt) by eauto.
+  eauto.
+  repeat erewrite (@eval_agree_in _ vs vt) by eauto.
+  eauto.
+
+  inversion H; unfold_all; subst.
+  descend.
+  econstructor.
+  repeat erewrite (@eval_agree_in _ vs vt') by eauto.
+  eauto.
+  repeat erewrite (@eval_agree_in _ vs vt') by eauto.
+  eauto.
+  eauto.
+
+  descend.
+  econstructor 14.
+  repeat erewrite (@eval_agree_in _ vs vt') by eauto.
+  eauto.
+  repeat erewrite (@eval_agree_in _ vs vt') by eauto.
+  eauto.
+  eauto.
+  eauto.
+
+Qed.
